Disjoint.v
@@ -2,11 +2,13 @@ From Coq Require Import Arith.Arith.
 From Coq Require Import Lia.
 
 From Elo Require Import Array.
+From Elo Require Import Map.
 From Elo Require Import Core0.
 From Elo Require Import Access.
 From Elo Require Import Compat.
 From Elo Require Import WBA.
 From Elo Require Import AccessProp.
+From Elo Require Import NoLoc.
 
 Definition disjoint_memory m ths := forall tid1 tid2 ad,
   access m (getTM ths tid1) ad ->
@@ -88,7 +90,7 @@ Proof.
                   inaccessible_address_set_2.
 Qed.
 
-Theorem disjoint_memory_preservation : forall m m' ths t' tid eff,
+Local Lemma disjoint_memory_preservation' : forall m m' ths t' tid eff,
   (forall tid, well_behaved_access m (getTM ths tid)) ->
   disjoint_memory m ths ->
   tid < length ths ->
@@ -100,5 +102,48 @@ Proof.
               alloc_disjoint_memory_preservation,
               load_disjoint_memory_preservation,
               store_disjoint_memory_preservation.
+Qed.
+
+Theorem disjoint_memory_preservation : forall m m' ths ths' tid eff,
+  (forall tid, SpawnNoLoc (getTM ths tid)) ->
+  (forall tid, well_behaved_access m (getTM ths tid)) ->
+  disjoint_memory m ths ->
+  tid < length ths ->
+  m / ths ~~[tid, eff]~~> m' / ths' ->
+  disjoint_memory m' ths'.
+Proof.
+  intros. inversion_cstep;
+  eauto using disjoint_memory_preservation'.
+  intros tid1 tid2 ad Hacc Hneq.
+  decompose sum (lt_eq_lt_dec (length ths) tid2); subst.
+  - rewrite (get_add_gt TM_Nil);
+    try solve [rewrite set_preserves_length; trivial].
+    intros ?. inversion_access.
+  - erewrite <- set_preserves_length.
+    rewrite (get_add_eq TM_Nil).
+    eauto using noloc_then_not_access, noloc_for_block.
+  - rewrite (get_add_lt TM_Nil);
+    try solve [rewrite set_preserves_length; trivial].
+    decompose sum (lt_eq_lt_dec (length ths) tid1); subst.
+    + rewrite (get_add_gt TM_Nil) in Hacc;
+      try solve [rewrite set_preserves_length; trivial].
+      inversion_access.
+    + erewrite <- set_preserves_length in Hacc.
+      rewrite (get_add_eq TM_Nil) in Hacc.
+      assert (~ access m' block ad) by 
+        eauto using noloc_then_not_access, noloc_for_block.
+      eauto.
+    + rewrite (get_add_lt TM_Nil) in Hacc;
+      try solve [rewrite set_preserves_length; trivial].
+      destruct (Nat.eq_dec tid tid1), (Nat.eq_dec tid tid2); subst; eauto.
+      * rewrite (get_set_neq TM_Nil); try lia.
+        rewrite (get_set_eq TM_Nil) in *; trivial.
+        eauto using step_spawn_inherits_access.
+      * rewrite (get_set_eq TM_Nil); trivial.
+        rewrite (get_set_neq TM_Nil) in *; trivial.
+        eauto using step_spawn_preserves_not_access.
+      * rewrite (get_set_neq TM_Nil); try lia.
+        rewrite (get_set_neq TM_Nil) in *; try lia.
+        eauto.
 Qed.
 
