Preservation.v
@@ -1,0 +1,122 @@
+From Coq Require Import Lia.
+
+From Elo Require Export Array.
+From Elo Require Export Map.
+From Elo Require Export Core0.
+
+Ltac splits n :=
+  match n with
+  | O => fail
+  | S O => idtac
+  | S ?n' => split; [| splits n']
+  end.
+
+(* ------------------------------------------------------------------------- *)
+(* Definitions ------------------------------------------------------------- *)
+(* ------------------------------------------------------------------------- *)
+
+Definition well_typed_memory mt m :=
+  length mt = length m /\
+  (forall ad, mt / empty |-- (getTM m ad) is (getTY mt ad)).
+
+Definition well_typed_threads mt ths :=
+  forall tid, exists T, mt / empty |-- (getTM ths tid) is T.
+
+Definition finished ths :=
+  forall tid, value (getTM ths tid).
+
+(* ------------------------------------------------------------------------- *)
+(* Extends ----------------------------------------------------------------- *)
+(* ------------------------------------------------------------------------- *)
+
+Module Extends.
+  Inductive extends' {A} : list A -> list A -> Prop :=
+    | extends_nil : forall mt,
+      extends' mt nil
+    | extends_cons : forall x mt mt',
+      extends' mt mt' ->
+      extends' (x :: mt) (x :: mt').
+
+    Infix "extends" := extends' (at level 50).
+
+    Lemma refl : forall {A} (mt : list A),
+      mt extends mt.
+    Proof.
+      intros. induction mt; eauto using @extends'.
+    Qed.
+
+    Lemma add : forall {A} (mt : list A) a,
+      (add mt a) extends mt.
+    Proof.
+      intros. induction mt; eauto using @extends'.
+    Qed.
+
+    Lemma get : forall (mt mt' : list typ) i,
+      i < length mt' ->
+      mt extends mt' ->
+      getTY mt' i = getTY mt i.
+    Proof.
+      intros *. generalize dependent mt. generalize dependent i.
+      induction mt'; intros * Hlen Hext; try solve [inversion Hlen].
+      inversion Hext; subst. destruct i; trivial.
+      unfold getTY, get. simpl in *. eauto using Lt.lt_S_n.
+    Qed.
+
+    Lemma length : forall {A} (mt mt' : list A) i,
+      i < length mt' ->
+      mt extends mt' ->
+      i < length mt.
+    Proof.
+      intros *. generalize dependent mt. generalize dependent i.
+      induction mt'; intros * Hlen Hext; try solve [inversion Hlen].
+      inversion Hext; subst. destruct i;
+      eauto using PeanoNat.Nat.lt_0_succ, Lt.lt_n_S, Lt.lt_S_n.
+    Qed.
+End Extends.
+
+Infix "extends" := Extends.extends' (at level 50).
+
+(* ------------------------------------------------------------------------- *)
+(* Weakening --------------------------------------------------------------- *)
+(* ------------------------------------------------------------------------- *)
+
+Lemma memory_weakening : forall mt mt' Gamma t T,
+  mt extends mt' ->
+  mt' / Gamma |-- t is T ->
+  mt  / Gamma |-- t is T.
+Proof.
+  intros * Hext Htype.
+  induction Htype; eauto using well_typed_term.
+  erewrite Extends.get; eauto using well_typed_term, Extends.length.
+Qed.
+
+Lemma threads_memory_weakening : forall mt mt' ths,
+  mt' extends mt ->
+  well_typed_threads mt ths ->
+  well_typed_threads mt' ths.
+Proof.
+  intros * Hext Hths. intros tid.
+  specialize (Hths tid) as [? ?]. eexists.
+  eauto using memory_weakening.
+Qed.
+
+Lemma context_weakening : forall mt Gamma Gamma' t T,
+  Gamma includes Gamma' ->
+  mt / Gamma' |-- t is T ->
+  mt / Gamma  |-- t is T.
+Proof.
+  intros * Hinc Htype.
+  generalize dependent Gamma.
+  induction Htype; intros * Hinc;
+  eauto 6 using @well_typed_term, safe_preserves_inclusion,
+    update_preserves_inclusion.
+Qed.
+
+Lemma context_weakening_empty : forall mt Gamma t T,
+  mt / empty |-- t is T ->
+  mt / Gamma |-- t is T.
+Proof.
+  intros * Htype.
+  eapply (context_weakening _ _ empty); auto.
+  discriminate.
+Qed.
